Merge syntax defs into syn.v files
No need for the split anymore.

theories/Dot/syn.v
@@ -1,4 +1,490 @@
-From D.Dot Require Export dot_syn.
+From stdpp Require Import strings.
+From D Require Export prelude tactics asubst_base.
+
+Definition label := string.
+
+Inductive tm : Type :=
+  | tv : vl_ -> tm
+  | tapp : tm -> tm -> tm
+  | tproj : tm -> label -> tm
+  | tskip : tm -> tm
+ with vl_ : Type :=
+  | var_vl : var -> vl_
+  | vnat : nat -> vl_
+  | vabs : tm -> vl_
+  | vobj : list (label * dm) -> vl_
+ with dm : Type :=
+  | dtysyn : ty -> dm
+  | dtysem : list vl_ -> stamp -> dm
+  | dvl : vl_ -> dm
+ with path : Type :=
+  | pv : vl_ -> path
+  | pself : path -> label -> path
+ with ty : Type :=
+  | TTop : ty
+  | TBot : ty
+  | TAnd : ty -> ty -> ty
+  | TOr : ty -> ty -> ty
+  | TLater : ty -> ty
+  | TAll : ty -> ty -> ty
+  | TMu : ty -> ty
+  | TVMem : label -> ty -> ty
+  | TTMem : label -> ty -> ty -> ty
+  | TSel : path -> label -> ty
+  | TNat : ty.
+
+Definition vl := vl_.
+
+Definition vls := list vl.
+Definition dms := list (label * dm).
+Definition ctx := list ty.
+
+Implicit Types
+         (T: ty) (v: vl) (t e: tm) (d: dm) (ds: dms) (vs: vls)
+         (Γ : ctx).
+
+Definition label_of_ty (T: ty): option label :=
+  match T with
+  | TTMem l _ _ => Some l
+  | TVMem l _ => Some l
+  | _ => None
+  end.
+
+Fixpoint dms_lookup (l : label) (ds : dms): option dm :=
+  match ds with
+  | [] => None
+  | (l', d) :: ds =>
+    match (decide (l = l')) with
+    | left Heq => Some d
+    | right _ => dms_lookup l ds
+    end
+  end.
+
+Definition dms_has ds l d := dms_lookup l ds = Some d.
+Definition dms_hasnt ds l := dms_lookup l ds = None.
+
+(* Module Coq_IndPrinciples_Bad. *)
+(*   Scheme tm_bad_mut_ind := Induction for tm Sort Prop *)
+(*   with   vl_bad_mut_ind := Induction for vl Sort Prop *)
+(*   with   dm_bad_mut_ind := Induction for dm Sort Prop *)
+(*   with   path_bad_mut_ind := Induction for path Sort Prop *)
+(*   with   ty_bad_mut_ind := Induction for ty Sort Prop. *)
+
+(*   Combined Scheme syntax_bad_mut_ind from tm_bad_mut_ind, vl_bad_mut_ind, dm_bad_mut_ind, path_bad_mut_ind, ty_bad_mut_ind. *)
+(*   Check syntax_bad_mut_ind. *)
+
+(*   Scheme tm_bad_mut_rect := Induction for tm Sort Type *)
+(*   with   vl_bad_mut_rect := Induction for vl Sort Type *)
+(*   with   dm_bad_mut_rect := Induction for dm Sort Type *)
+(*   with   path_bad_mut_rect := Induction for path Sort Type *)
+(*   with   ty_bad_mut_rect := Induction for ty Sort Type. *)
+
+(*   Fail Combined Scheme syntax_bad_mut_rect from tm_bad_mut_rect, vl_bad_mut_rect, dm_bad_mut_rect, path_bad_mut_rect, ty_bad_mut_rect. *)
+(*   Combined Scheme syntax_bad_mut_rect from tm_bad_mut_ind, vl_bad_mut_rect, dm_bad_mut_rect, path_bad_mut_rect, ty_bad_mut_rect. *)
+(*   Check syntax_bad_mut_rect. *)
+(* End Coq_IndPrinciples_Bad. *)
+
+Section syntax_mut_rect.
+  Variable Ptm : tm   → Type.
+  Variable Pvl : vl   → Type.
+  Variable Pdm : dm   → Type.
+  Variable Ppt : path → Type.
+  Variable Pty : ty   → Type.
+
+  Variable step_tv: ∀ v1, Pvl v1 → Ptm (tv v1).
+  Variable step_tapp: ∀ t1 t2, Ptm t1 → Ptm t2 → Ptm (tapp t1 t2).
+  Variable step_tproj: ∀ t1 l, Ptm t1 → Ptm (tproj t1 l).
+  Variable step_tskip: ∀ t1, Ptm t1 → Ptm (tskip t1).
+  Variable step_var_vl: ∀ i, Pvl (var_vl i).
+  Variable step_vnat: ∀ n, Pvl (vnat n).
+  Variable step_vabs: ∀ t1, Ptm t1 → Pvl (vabs t1).
+  (* Original: *)
+  (* Variable step_vobj: ∀ l, Pvl (vobj l). *)
+  Variable step_vobj: ∀ ds, ForallT Pdm (map snd ds) → Pvl (vobj ds).
+  Variable step_dtysyn: ∀ T1, Pty T1 → Pdm (dtysyn T1).
+  (* Original: *)
+  (* Variable step_dtysem: ∀ vsl g, Pdm (dtysem vs g). *)
+  Variable step_dtysem: ∀ vs s, ForallT Pvl vs → Pdm (dtysem vs s).
+  Variable step_dvl: ∀ v1, Pvl v1 → Pdm (dvl v1).
+  Variable step_pv: ∀ v1, Pvl v1 → Ppt (pv v1).
+  Variable step_psefl: ∀ p1 l, Ppt p1 → Ppt (pself p1 l).
+  Variable step_TTop: Pty TTop.
+  Variable step_TBot: Pty TBot.
+  Variable step_TAnd: ∀ T1 T2, Pty T1 → Pty T2 → Pty (TAnd T1 T2).
+  Variable step_TOr: ∀ T1 T2, Pty T1 → Pty T2 → Pty (TOr T1 T2).
+  Variable step_TLater: ∀ T1, Pty T1 → Pty (TLater T1).
+  Variable step_TAll: ∀ T1 T2, Pty T1 → Pty T2 → Pty (TAll T1 T2).
+  Variable step_TMu: ∀ T1, Pty T1 → Pty (TMu T1).
+  Variable step_TVMem: ∀ l T1, Pty T1 → Pty (TVMem l T1).
+  Variable step_TTMem: ∀ l T1 T2, Pty T1 → Pty T2 → Pty (TTMem l T1 T2).
+  Variable step_TSel: ∀ p1 l, Ppt p1 → Pty (TSel p1 l).
+  Variable step_TNat: Pty TNat.
+
+  Fixpoint tm_mut_rect t: Ptm t
+  with vl_mut_rect v: Pvl v
+  with dm_mut_rect d: Pdm d
+  with path_mut_rect p: Ppt p
+  with ty_mut_rect T: Pty T.
+  Proof.
+    (* Automation risk producing circular proofs that call right away the lemma we're proving.
+       Instead we want to apply one of the [case_] arguments to perform an
+       inductive step, and only then call ourselves recursively. *)
+    all: destruct 0;
+      try match goal with
+      (* Warning: add other arities as needed. *)
+      | Hstep: context [?P (?c _ _ _ _)] |- ?P (?c _ _ _ _) => apply Hstep; trivial
+      | Hstep: context [?P (?c _ _ _)] |- ?P (?c _ _ _) => apply Hstep; trivial
+      | Hstep: context [?P (?c _ _)] |- ?P (?c _ _) => apply Hstep; trivial
+      | Hstep: context [?P (?c _)] |- ?P (?c _) => apply Hstep; trivial
+      | Hstep: context [?P (?c)] |- ?P (?c) => apply Hstep; trivial
+      end.
+    - elim: l => [|[l d] ds IHds] //=; auto.
+    - elim: l => [|v vs IHxs] //=; auto.
+  Qed.
+
+  Lemma syntax_mut_rect: (∀ t, Ptm t) * (∀ v, Pvl v) * (∀ d, Pdm d) * (∀ p, Ppt p) * (∀ T, Pty T).
+  Proof.
+    repeat split; intros.
+    - eapply tm_mut_rect.
+    - eapply vl_mut_rect.
+    - eapply dm_mut_rect.
+    - eapply path_mut_rect.
+    - eapply ty_mut_rect.
+  Qed.
+End syntax_mut_rect.
+
+Section syntax_mut_ind.
+  Variable Ptm : tm   → Prop.
+  Variable Pvl : vl   → Prop.
+  Variable Pdm : dm   → Prop.
+  Variable Ppt : path → Prop.
+  Variable Pty : ty   → Prop.
+
+  Variable step_tv: ∀ v1, Pvl v1 → Ptm (tv v1).
+  Variable step_tapp: ∀ t1 t2, Ptm t1 → Ptm t2 → Ptm (tapp t1 t2).
+  Variable step_tproj: ∀ t1 l, Ptm t1 → Ptm (tproj t1 l).
+  Variable step_tskip: ∀ t1, Ptm t1 → Ptm (tskip t1).
+  Variable step_var_vl: ∀ i, Pvl (var_vl i).
+  Variable step_vnat: ∀ n, Pvl (vnat n).
+  Variable step_vabs: ∀ t1, Ptm t1 → Pvl (vabs t1).
+  (* Original: *)
+  (* Variable step_vobj: ∀ l, Pvl (vobj l). *)
+  Variable step_vobj: ∀ ds, Forall Pdm (map snd ds) → Pvl (vobj ds).
+  Variable step_dtysyn: ∀ T1, Pty T1 → Pdm (dtysyn T1).
+  (* Original: *)
+  (* Variable step_dtysem: ∀ vsl g, Pdm (dtysem vs g). *)
+  Variable step_dtysem: ∀ vs s, Forall Pvl vs → Pdm (dtysem vs s).
+  Variable step_dvl: ∀ v1, Pvl v1 → Pdm (dvl v1).
+  Variable step_pv: ∀ v1, Pvl v1 → Ppt (pv v1).
+  Variable step_psefl: ∀ p1 l, Ppt p1 → Ppt (pself p1 l).
+  Variable step_TTop: Pty TTop.
+  Variable step_TBot: Pty TBot.
+  Variable step_TAnd: ∀ T1 T2, Pty T1 → Pty T2 → Pty (TAnd T1 T2).
+  Variable step_TOr: ∀ T1 T2, Pty T1 → Pty T2 → Pty (TOr T1 T2).
+  Variable step_TLater: ∀ T1, Pty T1 → Pty (TLater T1).
+  Variable step_TAll: ∀ T1 T2, Pty T1 → Pty T2 → Pty (TAll T1 T2).
+  Variable step_TMu: ∀ T1, Pty T1 → Pty (TMu T1).
+  Variable step_TVMem: ∀ l T1, Pty T1 → Pty (TVMem l T1).
+  Variable step_TTMem: ∀ l T1 T2, Pty T1 → Pty T2 → Pty (TTMem l T1 T2).
+  Variable step_TSel: ∀ p1 l, Ppt p1 → Pty (TSel p1 l).
+  Variable step_TNat: Pty TNat.
+
+  Lemma syntax_mut_ind: (∀ t, Ptm t) ∧ (∀ v, Pvl v) ∧ (∀ d, Pdm d) ∧ (∀ p, Ppt p) ∧ (∀ T, Pty T).
+  Proof.
+    efeed pose proof syntax_mut_rect as H; try done.
+    - intros ds HdsT. apply step_vobj, ForallT_Forall, HdsT.
+    - intros vs g HvsT. apply step_dtysem, ForallT_Forall, HvsT.
+    - ev; split_and! ; assumption.
+  Qed.
+End syntax_mut_ind.
+
+Instance inh_ty : Inhabited ty := populate TNat.
+Instance inh_vl : Inhabited vl := populate (vnat 0).
+Instance inh_dm : Inhabited dm := populate (dvl inhabitant).
+Instance inh_pth : Inhabited path := populate (pv inhabitant).
+Instance inh_tm : Inhabited tm := populate (tv inhabitant).
+
+Instance ids_vl : Ids vl := var_vl.
+
+Instance inj_ids : Inj (=) (=@{vl}) ids.
+Proof. by move=>??[]. Qed.
+
+Instance ids_tm : Ids tm := inh_ids.
+Instance ids_dm : Ids dm := inh_ids.
+Instance ids_pth : Ids path := inh_ids.
+Instance ids_ty : Ids ty := inh_ids.
+Instance ids_vls : Ids vls := _.
+Instance ids_dms : Ids dms := _.
+Instance ids_ctx : Ids ctx := _.
+
+Fixpoint tm_rename (sb : var → var) (e : tm) {struct e} : tm :=
+  let a := tm_rename : Rename tm in
+  let b := vl_rename : Rename vl in
+  match e with
+  | tv v => tv (rename sb v)
+  | tapp t1 t2 => tapp (rename sb t1) (rename sb t2)
+  | tproj t l => (tproj (rename sb t) l)
+  | tskip t => tskip (rename sb t)
+  end
+with
+vl_rename (sb : var → var) (v : vl) {struct v} : vl :=
+  let a := tm_rename : Rename tm in
+  let b := vl_rename : Rename vl in
+  let c := dm_rename : Rename dm in
+  match v with
+  | var_vl x => var_vl (sb x)
+  | vnat n => vnat n
+  | vabs t => vabs (rename (upren sb) t)
+  | vobj d => vobj (rename (upren sb) d)
+  end
+with
+dm_rename (sb : var → var) (d : dm) {struct d} : dm :=
+  let a := vl_rename : Rename vl in
+  let b := ty_rename : Rename ty in
+  match d with
+  | dtysyn ty => dtysyn (rename sb ty)
+  | dtysem lv γ => dtysem (rename sb lv) γ
+  | dvl v => dvl (rename sb v)
+  end
+with
+ty_rename (sb : var → var) (T : ty) {struct T}: ty :=
+  let a := ty_rename : Rename ty in
+  let b := path_rename : Rename path in
+  match T with
+  | TTop => TTop
+  | TBot => TBot
+  | TAnd T1 T2 => TAnd (rename sb T1) (rename sb T2)
+  | TOr T1 T2 => TOr (rename sb T1) (rename sb T2)
+  | TLater T => TLater (rename sb T)
+  | TAll T1 T2 => TAll (rename sb T1) (rename (upren sb) T2)
+  | TMu T => TMu (rename (upren sb) T)
+  | TVMem l T => TVMem l (rename sb T)
+  | TTMem l T1 T2 => TTMem l (rename sb T1) (rename sb T2)
+  | TSel pth l => TSel (rename sb pth) l
+  | TNat => TNat
+  end
+with
+path_rename (sb : var → var) (pth : path) {struct pth} : path :=
+  let a := vl_rename : Rename vl in
+  let b := path_rename : Rename path in
+  match pth with
+  | pv v => pv (rename sb v)
+  | pself pth l => pself (rename sb pth) l
+  end.
+
+Instance rename_tm : Rename tm := tm_rename.
+Instance rename_vl : Rename vl := vl_rename.
+Instance rename_ty : Rename ty := ty_rename.
+Instance rename_dm : Rename dm := dm_rename.
+Instance rename_pth : Rename path := path_rename.
+
+Hint Rewrite @list_rename_fold @list_pair_rename_fold : autosubst.
+
+Fixpoint tm_hsubst (sb : var → vl) (e : tm) : tm :=
+  let a := tm_hsubst : HSubst vl tm in
+  let b := vl_subst : Subst vl in
+  match e with
+  | tv v => tv (subst sb v)
+  | tapp t1 t2 => tapp (hsubst sb t1) (hsubst sb t2)
+  | tproj t l => (tproj (hsubst sb t) l)
+  | tskip t => tskip (hsubst sb t)
+  end
+with
+vl_subst (sb : var → vl) (v : vl) : vl :=
+  let a := tm_hsubst : HSubst vl tm in
+  let b := dm_hsubst : HSubst vl dm in
+  match v with
+  | var_vl x => sb x
+  | vnat n => vnat n
+  | vabs t => vabs (hsubst (up sb) t)
+  | vobj d => vobj (hsubst (up sb) d)
+  end
+with
+dm_hsubst (sb : var → vl) (d : dm) : dm :=
+  let a := vl_subst : Subst vl in
+  let b := ty_hsubst : HSubst vl ty in
+  match d with
+  | dtysyn ty => dtysyn (hsubst sb ty)
+  | dtysem lv γ => dtysem (hsubst sb lv) γ
+  | dvl v => dvl (subst sb v)
+  end
+with
+ty_hsubst (sb : var → vl) (T : ty) : ty :=
+  let a := ty_hsubst : HSubst vl ty in
+  let b := path_hsubst : HSubst vl path in
+  match T with
+  | TTop => TTop
+  | TBot => TBot
+  | TAnd T1 T2 => TAnd (hsubst sb T1) (hsubst sb T2)
+  | TOr T1 T2 => TOr (hsubst sb T1) (hsubst sb T2)
+  | TLater T => TLater (hsubst sb T)
+  | TAll T1 T2 => TAll (hsubst sb T1) (hsubst (up sb) T2)
+  | TMu T => TMu (hsubst (up sb) T)
+  | TVMem l T => TVMem l (hsubst sb T)
+  | TTMem l T1 T2 => TTMem l (hsubst sb T1) (hsubst sb T2)
+  | TSel pth l => TSel (hsubst sb pth) l
+  | TNat => TNat
+  end
+with
+path_hsubst (sb : var → vl) (pth : path) : path :=
+  let b := vl_subst : Subst vl in
+  let b := path_hsubst : HSubst vl path in
+  match pth with
+  | pv v => pv (subst sb v)
+  | pself pth l => pself (hsubst sb pth) l
+  end.
+
+Instance subst_vl : Subst vl := vl_subst.
+Instance hsubst_tm : HSubst vl tm := tm_hsubst.
+Instance hsubst_ty : HSubst vl ty := ty_hsubst.
+Instance hsubst_dm : HSubst vl dm := dm_hsubst.
+Instance hsubst_pth : HSubst vl path := path_hsubst.
+
+Lemma vl_eq_dec (v1 v2 : vl) : Decision (v1 = v2)
+with
+tm_eq_dec (t1 t2 : tm) : Decision (t1 = t2)
+with
+dm_eq_dec (d1 d2 : dm) : Decision (d1 = d2)
+with
+ty_eq_dec (ty1 ty2 : ty) : Decision (ty1 = ty2)
+with
+path_eq_dec (pth1 pth2 : path) : Decision (pth1 = pth2).
+Proof.
+   all: rewrite /Decision; decide equality;
+       try repeat (apply vl_eq_dec || apply tm_eq_dec || apply ty_eq_dec || apply path_eq_dec ||
+            apply @prod_eq_dec ||
+            apply @list_eq_dec ||
+            apply nat_eq_dec || apply positive_eq_dec || apply string_eq_dec); auto.
+Qed.
+
+Instance vl_eq_dec' : EqDecision vl := vl_eq_dec.
+Instance tm_eq_dec' : EqDecision tm := tm_eq_dec.
+Instance dm_eq_dec' : EqDecision dm := dm_eq_dec.
+Instance ty_eq_dec' : EqDecision ty := ty_eq_dec.
+Instance path_eq_dec' : EqDecision path := path_eq_dec.
+Instance vls_eq_dec' : EqDecision vls := list_eq_dec.
+Instance dms_eq_dec' : EqDecision dms := list_eq_dec.
+
+Local Ltac finish_lists l x :=
+  elim: l => [|x xs IHds] //=; idtac + elim: x => [l d] //=; f_equal => //; by f_equal.
+
+Lemma vl_rename_Lemma (ξ : var → var) (v : vl) : rename ξ v = v.[ren ξ]
+with
+tm_rename_Lemma (ξ : var → var) (t : tm) : rename ξ t = t.|[ren ξ]
+with
+dm_rename_Lemma (ξ : var → var) (d : dm) : rename ξ d = d.|[ren ξ]
+with
+ty_rename_Lemma (ξ : var → var) (T : ty) : rename ξ T = T.|[ren ξ]
+with
+path_rename_Lemma (ξ : var → var) (pth : path) :
+  rename ξ pth = pth.|[ren ξ].
+Proof.
+  all: destruct 0; rewrite /= ?up_upren_internal; f_equal => //; finish_lists l x.
+Qed.
+
+Lemma vl_ids_Lemma (v : vl) : v.[ids] = v
+with
+tm_ids_Lemma (t : tm) : t.|[ids] = t
+with
+dm_ids_Lemma (d : dm) : d.|[ids] = d
+with
+ty_ids_Lemma (T : ty) : T.|[ids] = T
+with
+path_ids_Lemma (pth : path) : pth.|[ids] = pth.
+Proof.
+  all: destruct 0; rewrite /= ?up_id_internal; f_equal => //; finish_lists l x.
+Qed.
+
+Lemma vl_comp_rename_Lemma (ξ : var → var) (σ : var → vl) (v : vl) :
+  (rename ξ v).[σ] = v.[ξ >>> σ]
+with
+tm_comp_rename_Lemma (ξ : var → var) (σ : var → vl) (t : tm) :
+  (rename ξ t).|[σ] = t.|[ξ >>> σ]
+with
+dm_comp_rename_Lemma (ξ : var → var) (σ : var → vl) (d : dm) :
+  (rename ξ d).|[σ] = d.|[ξ >>> σ]
+with
+ty_comp_rename_Lemma (ξ : var → var) (σ : var → vl) (T : ty) :
+  (rename ξ T).|[σ] = T.|[ξ >>> σ]
+with
+path_comp_rename_Lemma (ξ : var → var) (σ : var → vl) (pth : path) :
+  (rename ξ pth).|[σ] = pth.|[ξ >>> σ].
+Proof.
+  all: destruct 0; rewrite /= 1? up_comp_ren_subst; f_equal => //; finish_lists l x.
+Qed.
+
+Lemma vl_rename_comp_Lemma (σ : var → vl) (ξ : var → var) (v : vl) :
+  rename ξ v.[σ] = v.[σ >>> rename ξ]
+with
+tm_rename_comp_Lemma (σ : var → vl) (ξ : var → var) (t : tm) :
+  rename ξ t.|[σ] = t.|[σ >>> rename ξ]
+with
+dm_rename_comp_Lemma (σ : var → vl) (ξ : var → var) (d : dm) :
+  rename ξ d.|[σ] = d.|[σ >>> rename ξ]
+with
+ty_rename_comp_Lemma (σ : var → vl) (ξ : var → var) (T : ty) :
+  rename ξ T.|[σ] = T.|[σ >>> rename ξ]
+with
+path_rename_comp_Lemma (σ : var → vl) (ξ : var → var) (pth : path) :
+  rename ξ pth.|[σ] = pth.|[σ >>> rename ξ].
+Proof.
+  all: destruct 0; rewrite /= ? up_comp_subst_ren_internal; f_equal => //;
+    auto using vl_rename_Lemma, vl_comp_rename_Lemma; finish_lists l x.
+Qed.
+
+Lemma vl_comp_Lemma (σ τ : var → vl) (v : vl) : v.[σ].[τ] = v.[σ >> τ]
+with
+tm_comp_Lemma (σ τ : var → vl) (t : tm) : t.|[σ].|[τ] = t.|[σ >> τ]
+with
+dm_comp_Lemma (σ τ : var → vl) (d : dm) : d.|[σ].|[τ] = d.|[σ >> τ]
+with
+ty_comp_Lemma (σ τ : var → vl) (T : ty) : T.|[σ].|[τ] = T.|[σ >> τ]
+with
+path_comp_Lemma (σ τ : var → vl) (pth : path) : pth.|[σ].|[τ] = pth.|[σ >> τ].
+Proof.
+  all: destruct 0; rewrite /= ? up_comp_internal; f_equal;
+    auto using vl_rename_comp_Lemma, vl_comp_rename_Lemma; finish_lists l x.
+Qed.
+
+Instance subst_lemmas_vl : SubstLemmas vl.
+Proof.
+  split; auto using vl_rename_Lemma, vl_ids_Lemma, vl_comp_Lemma.
+Qed.
+
+Instance hsubst_lemmas_tm : HSubstLemmas vl tm.
+Proof.
+  split; auto using tm_ids_Lemma, tm_comp_Lemma.
+Qed.
+
+Instance hsubst_lemmas_ty : HSubstLemmas vl ty.
+Proof.
+  split; auto using ty_ids_Lemma, ty_comp_Lemma.
+Qed.
+
+Instance hsubst_lemmas_dm : HSubstLemmas vl dm.
+Proof.
+  split; auto using dm_ids_Lemma, dm_comp_Lemma.
+Qed.
+
+Instance hsubst_lemmas_pth : HSubstLemmas vl path.
+Proof.
+  split; auto using path_ids_Lemma, path_comp_Lemma.
+Qed.
+
+Instance hsubst_lemmas_vls : HSubstLemmas vl vls := _.
+
+Instance hsubst_lemmas_ctx : HSubstLemmas vl ctx := _.
+
+Instance inh_string: Inhabited string := populate "".
+Instance inh_label: Inhabited label := _.
+Instance hsubst_lemmas_dms : HSubstLemmas vl dms := _.
+
+Include Sorts.
+
+Instance sort_tm: Sort tm := {}.
+Instance sort_dm: Sort dm := {}.
+Instance sort_path: Sort path := {}.
+Instance sort_ty: Sort ty := {}.
 
 (** After instantiating Autosubst, a few binding-related syntactic definitions
     that need not their own file. *)
